SHA2_384: align the bundle signatures with the verified module

code/hash/SHA2_384.fst
@@ -13,6 +13,7 @@ open FStar.Buffer
 open Hacl.Cast
 open Hacl.UInt8
 open Hacl.UInt32
+open Hacl.Spec.Endianness
 open FStar.UInt32
 
 open Hacl.Hash.SHA2_384
@@ -55,7 +56,7 @@ let size_block = Hash.size_block
 let size_state = Hash.size_state
 
 
-#reset-options "--max_fuel 0  --z3rlimit 10"
+#reset-options "--max_fuel 0  --z3rlimit 25"
 
 [@"c_inline"]
 val alloc:
@@ -68,7 +69,7 @@ val alloc:
 let alloc () = Hash.alloc ()
 
 
-#reset-options "--max_fuel 0  --z3rlimit 30"
+#reset-options "--max_fuel 0  --z3rlimit 25"
 
 val init:
   state:uint64_p{length state = v size_state} ->
@@ -82,14 +83,14 @@ val init:
               let slice_h_0 = Seq.slice (as_seq h1 state) (U32.v pos_whash_w) (U32.(v pos_whash_w + v size_whash_w)) in
               let seq_counter = Seq.slice (as_seq h1 state) (U32.v pos_count_w) (U32.(v pos_count_w + v size_count_w)) in
               let counter = Seq.index seq_counter 0 in
-              let seq_k = Hacl.Spec.Endianness.reveal_h64s slice_k in
-              let seq_h_0 = Hacl.Spec.Endianness.reveal_h64s slice_h_0 in
+              let seq_k = reveal_h64s slice_k in
+              let seq_h_0 = reveal_h64s slice_h_0 in
               seq_k == Spec.k /\ seq_h_0 == Spec.h_0 /\ H64.v counter = 0)))
 
 let init state = Hash.init state
 
 
-#reset-options "--max_fuel 0  --z3rlimit 50"
+#reset-options "--max_fuel 0  --z3rlimit 25"
 
 val update:
   state :uint64_p {length state = v size_state} ->
@@ -99,7 +100,7 @@ val update:
                   /\ (let seq_k = Seq.slice (as_seq h0 state) (U32.v pos_k_w) (U32.(v pos_k_w + v size_k_w)) in
                   let seq_counter = Seq.slice (as_seq h0 state) (U32.v pos_count_w) (U32.(v pos_count_w + v size_count_w)) in
                   let counter = Seq.index seq_counter 0 in
-                  seq_k == Spec.k /\ H64.v counter < (pow2 32 - 1))))
+                  reveal_h64s seq_k == Spec.k /\ H64.v counter < (pow2 64 - 1))))
         (ensures  (fun h0 r h1 -> live h0 state /\ live h0 data /\ live h1 state /\ modifies_1 state h0 h1
                   /\ (let seq_hash_0 = Seq.slice (as_seq h0 state) (U32.v pos_whash_w) (U32.(v pos_whash_w + v size_whash_w)) in
                   let seq_hash_1 = Seq.slice (as_seq h1 state) (U32.v pos_whash_w) (U32.(v pos_whash_w + v size_whash_w)) in
@@ -111,37 +112,39 @@ val update:
                   let counter_0 = Seq.index seq_counter_0 0 in
                   let counter_1 = Seq.index seq_counter_1 0 in
                   seq_k_0 == seq_k_1
-                  /\ H64.v counter_1 = H64.v counter_0 + 1 /\ H64.v counter_1 < pow2 32
-                  /\ seq_hash_1 == Spec.update seq_hash_0 seq_block)))
+                  /\ H64.v counter_1 = H64.v counter_0 + 1 /\ H64.v counter_1 < pow2 64
+                  /\ reveal_h64s seq_hash_1 == Spec.update (reveal_h64s seq_hash_0) (reveal_sbytes seq_block))))
 
 let update state data_8 = Hash.update state data_8
 
 
-#reset-options "--max_fuel 0  --z3rlimit 100"
+#reset-options "--max_fuel 0  --z3rlimit 25"
 
 val update_multi:
   state :uint64_p{length state = v size_state} ->
   data  :uint8_p {length data % v size_block = 0 /\ disjoint state data} ->
   n     :uint32_t{v n * v size_block = length data} ->
   Stack unit
-        (requires (fun h0 -> live h0 state /\ live h0 data
-                  /\ (let seq_k = Seq.slice (as_seq h0 state) (U32.v pos_k_w) (U32.(v pos_k_w + v size_k_w)) in
+        (requires (fun h0 -> live h0 state /\ live h0 data /\
+                 (let seq_k = Seq.slice (as_seq h0 state) (U32.v pos_k_w) (U32.(v pos_k_w + v size_k_w)) in
                   let seq_counter = Seq.slice (as_seq h0 state) (U32.v pos_count_w) (U32.(v pos_count_w + v size_count_w)) in
                   let counter = Seq.index seq_counter 0 in
-                  seq_k == Spec.k /\ H64.v counter < (pow2 32 - (v n)))))
-        (ensures  (fun h0 _ h1 -> live h0 state /\ live h0 data /\ live h1 state /\ modifies_1 state h0 h1
-                  /\ (let seq_hash_0 = Seq.slice (as_seq h0 state) (U32.v pos_whash_w) (U32.(v pos_whash_w + v size_whash_w)) in
-                  let seq_hash_1 = Seq.slice (as_seq h1 state) (U32.v pos_whash_w) (U32.(v pos_whash_w + v size_whash_w)) in
-                  let seq_k_0 = Seq.slice (as_seq h0 state) (U32.v pos_k_w) (U32.(v pos_k_w + v size_k_w)) in
-                  let seq_k_1 = Seq.slice (as_seq h1 state) (U32.v pos_k_w) (U32.(v pos_k_w + v size_k_w)) in
+                  reveal_h64s seq_k == Spec.k /\ H64.v counter < pow2 64 - (v n))))
+        (ensures  (fun h0 _ h1 -> live h0 state /\ live h0 data /\ live h1 state /\ modifies_1 state h0 h1 /\
+                 (let seq_hash0 = Seq.slice (as_seq h0 state) (U32.v pos_whash_w) (U32.(v pos_whash_w + v size_whash_w)) in
+                  let seq_hash1 = Seq.slice (as_seq h1 state) (U32.v pos_whash_w) (U32.(v pos_whash_w + v size_whash_w)) in
+                  let seq_k0 = Seq.slice (as_seq h0 state) (U32.v pos_k_w) (U32.(v pos_k_w + v size_k_w)) in
+                  let seq_k1 = Seq.slice (as_seq h1 state) (U32.v pos_k_w) (U32.(v pos_k_w + v size_k_w)) in
                   let seq_blocks = as_seq h0 data in
-                  let seq_counter_0 = Seq.slice (as_seq h0 state) (U32.v pos_count_w) (U32.(v pos_count_w + v size_count_w)) in
-                  let seq_counter_1 = Seq.slice (as_seq h1 state) (U32.v pos_count_w) (U32.(v pos_count_w + v size_count_w)) in
-                  let counter_0 = Seq.index seq_counter_0 0 in
-                  let counter_1 = Seq.index seq_counter_1 0 in
-                  seq_k_0 == seq_k_1
-                  /\ H64.v counter_1 = H64.v counter_0 + (v n) /\ H64.v counter_1 < pow2 32
-                  /\ seq_hash_1 == Spec.update_multi seq_hash_0 seq_blocks)))
+                  let seq_counter0 = Seq.slice (as_seq h0 state) (U32.v pos_count_w) (U32.(v pos_count_w + v size_count_w)) in
+                  let seq_counter1 = Seq.slice (as_seq h1 state) (U32.v pos_count_w) (U32.(v pos_count_w + v size_count_w)) in
+                  let counter0 = Seq.index seq_counter0 0 in
+                  let counter1 = Seq.index seq_counter1 0 in
+                  seq_k0 == seq_k1 /\
+                  H64.v counter1 = H64.v counter0 + (v n) /\
+                  H64.v counter1 < pow2 64 /\
+                  reveal_h64s seq_hash1 ==
+                  Spec.update_multi (reveal_h64s seq_hash0) (reveal_sbytes seq_blocks) )))
 
 let update_multi state data n = Hash.update_multi state data n
 
@@ -158,44 +161,45 @@ val update_last:
                   let seq_counter = Seq.slice (as_seq h0 state) (U32.v pos_count_w) (U32.(v pos_count_w + v size_count_w)) in
                   let counter = Seq.index seq_counter 0 in
                   let nb = U64.div len (u32_to_u64 size_block) in
-                  seq_k == Spec.k /\ H64.v counter < (pow2 32 - 2))))
+                  reveal_h64s seq_k == Spec.k /\ H64.v counter < (pow2 64 - 2))))
         (ensures  (fun h0 r h1 -> live h0 state /\ live h0 data /\ live h1 state /\ modifies_1 state h0 h1
                   /\ (let seq_hash_0 = Seq.slice (as_seq h0 state) (U32.v pos_whash_w) (U32.(v pos_whash_w + v size_whash_w)) in
                   let seq_hash_1 = Seq.slice (as_seq h1 state) (U32.v pos_whash_w) (U32.(v pos_whash_w + v size_whash_w)) in
-                  let seq_data = as_seq h0 data in
+                  let seq_data = reveal_sbytes (as_seq h0 data) in
                   let count = Seq.slice (as_seq h0 state) (U32.v pos_count_w) (U32.v pos_count_w + 1) in
-                  let prevlen = U32.(H64.v (Seq.index count 0) * (v size_block)) in
-                  seq_hash_1 == Spec.update_last seq_hash_0 prevlen seq_data)))
+                  let prevlen = H64.((H64.v (Seq.index count 0)) * (U32.v size_block)) in
+                  reveal_h64s seq_hash_1 == Spec.update_last (reveal_h64s seq_hash_0) prevlen seq_data)))
 
 let update_last state data len = Hash.update_last state data len
 
 
-#reset-options "--max_fuel 0  --z3rlimit 10"
+#reset-options "--max_fuel 0  --z3rlimit 25"
 
 val finish:
   state :uint64_p{length state = v size_state} ->
-  hash  :uint8_p{length hash = v size_hash} ->
+  hash  :uint8_p{length hash = v size_hash_final /\ disjoint state hash} ->
   Stack unit
         (requires (fun h0 -> live h0 state /\ live h0 hash))
-        (ensures  (fun h0 _ h1 -> live h0 state /\ live h1 hash /\ modifies_1 hash h0 h1
+        (ensures  (fun h0 _ h1 -> live h1 state /\ live h0 state
+                  /\ live h1 hash /\ live h0 hash /\ modifies_1 hash h0 h1
                   /\ (let seq_hash_w = Seq.slice (as_seq h0 state) (U32.v pos_whash_w) (U32.(v pos_whash_w + v size_whash_w)) in
-                  let seq_hash = as_seq h1 hash in
-                  seq_hash = Spec.finish seq_hash_w)))
+                  let seq_hash = reveal_sbytes (as_seq h1 hash) in
+                  seq_hash == Spec.finish (reveal_h64s seq_hash_w))))
 
 let finish state hash = Hash.finish state hash
 
 
-#reset-options "--max_fuel 0  --z3rlimit 10"
+#reset-options "--max_fuel 0  --z3rlimit 25"
 
 val hash:
-  hash :uint8_p {length hash = v size_hash} ->
-  input:uint8_p {length input < Spec.max_input_len_8} ->
+  hash :uint8_p {length hash = v size_hash_final} ->
+  input:uint8_p {length input < Spec.max_input_len_8 /\ disjoint hash input} ->
   len  :uint32_t{v len = length input} ->
   Stack unit
         (requires (fun h0 -> live h0 hash /\ live h0 input))
         (ensures  (fun h0 _ h1 -> live h0 input /\ live h0 hash /\ live h1 hash /\ modifies_1 hash h0 h1
-                  /\ (let seq_input = as_seq h0 input in
-                  let seq_hash = as_seq h1 hash in
+                  /\ (let seq_input = reveal_sbytes (as_seq h0 input) in
+                  let seq_hash = reveal_sbytes (as_seq h1 hash) in
                   seq_hash == Spec.hash seq_input)))
 
 let hash hash input len = Hash.hash hash input len
